Machine run unique result

theories/machine_run.v
@@ -2,145 +2,167 @@ From stdpp Require Import base.
 From iris.program_logic Require Import language.
 From cap_machine Require Import machine_parameters machine_base cap_lang.
 
-(* The operational semantics as an interpreter: this effectively "runs" the
-   machine until it fails or halts (or we run out of fuel). *)
+Section machine_run.
+  Context `{MachineParameters}.
 
-Fixpoint machine_run `{MachineParameters} (fuel: nat) (c: Conf): option ConfFlag :=
-  match fuel with
-  | 0 => None
-  | S fuel =>
-    match c with
-    | (Failed, _) => Some Failed
-    | (Halted, _) => Some Halted
-    | (NextI, φ) => machine_run fuel (Executable, φ)
-    | (Executable, (r, m)) =>
-      match r !! PC with
-      | None => Some Failed
-      | Some pc =>
-        if isCorrectPCb pc then (
-          let a := match pc with
-                  | WCap _ _ _ a => a
-                  | _ => top (* dummy *)
-                  end in
-          match m !! a with
-          | None => Some Failed
-          | Some wa =>
-              let i := decodeInstrW wa in
-              let c' := exec i (r, m) in
-              machine_run fuel (c'.1, c'.2)
-          end
-        ) else (
-          Some Failed
-        )
+  (* The operational semantics as an interpreter: this effectively "runs" the
+    machine until it fails or halts (or we run out of fuel). *)
+
+  Fixpoint machine_run (fuel: nat) (c: Conf): option ConfFlag :=
+    match fuel with
+    | 0 => None
+    | S fuel =>
+      match c with
+      | (Failed, _) => Some Failed
+      | (Halted, _) => Some Halted
+      | (NextI, φ) => machine_run fuel (Executable, φ)
+      | (Executable, (r, m)) =>
+        match r !! PC with
+        | None => Some Failed
+        | Some pc =>
+          if isCorrectPCb pc then (
+            let a := match pc with
+                    | WInt _ => top (* dummy *)
+                    | WCap _ _ _ a => a
+                    end in
+            match m !! a with
+            | None => Some Failed
+            | Some wa =>
+                let i := decodeInstrW wa in
+                let c' := exec i (r, m) in
+                machine_run fuel (c'.1, c'.2)
+            end
+          ) else (
+            Some Failed
+          )
+        end
       end
-    end
-  end.
+    end.
 
-Lemma machine_run_correct `{MachineParameters} fuel cf (φ: ExecConf) cf':
-  machine_run fuel (cf, φ) = Some cf' →
-  ∃ φ', rtc erased_step
-            ([Seq (Instr cf)], φ)
-            ([Instr cf'], φ').
-Proof.
-  revert cf cf' φ. induction fuel.
-  { cbn. done. }
-  { cbn. intros ? ? [r m] Hc.
-    destruct cf; simplify_eq.
-    destruct (r !! PC) as [wpc | ] eqn:HePC.
-    2: {
-      eexists. eapply rtc_l. unfold erased_step. exists [].
-      eapply step_atomic with (t1:=[]). 1,2: reflexivity. cbn.
-      eapply ectx_language.Ectx_step with (K:=[SeqCtx]). 1,2: reflexivity. cbn.
-      constructor. constructor; auto.
-      eapply rtc_once. exists []. simplify_eq.
-      eapply step_atomic with (t1:=[]). 1,2: reflexivity. cbn.
-      eapply ectx_language.Ectx_step with (K:=[]). 1,2: reflexivity. cbn.
-      constructor. }
-    destruct (isCorrectPCb wpc) eqn:HPC.
-    { apply isCorrectPCb_isCorrectPC in HPC.
-      destruct wpc eqn:Hr; [by inversion HPC| | by inversion HPC]. destruct sb as [p b e a | ]; last by inversion HPC.
-      destruct (m !! a) as [wa | ] eqn:HeMem.
+  Lemma machine_run_correct fuel cf (φ: ExecConf) cf':
+    machine_run fuel (cf, φ) = Some cf' →
+    ∃ φ', rtc erased_step
+              ([Seq (Instr cf)], φ)
+              ([Instr cf'], φ').
+  Proof.
+    revert cf cf' φ. induction fuel.
+    { cbn. done. }
+    { cbn. intros ? ? [r m] Hc.
+      destruct cf; simplify_eq.
+      destruct (r !! PC) as [wpc | ] eqn:HePC.
       2: {
         eexists. eapply rtc_l. unfold erased_step. exists [].
         eapply step_atomic with (t1:=[]). 1,2: reflexivity. cbn.
         eapply ectx_language.Ectx_step with (K:=[SeqCtx]). 1,2: reflexivity. cbn.
-        constructor. eapply step_exec_memfail; eauto.
+        constructor. constructor; auto.
         eapply rtc_once. exists []. simplify_eq.
         eapply step_atomic with (t1:=[]). 1,2: reflexivity. cbn.
         eapply ectx_language.Ectx_step with (K:=[]). 1,2: reflexivity. cbn.
         constructor. }
-      eapply IHfuel in Hc as [φ' Hc]. eexists.
-      eapply rtc_l. unfold erased_step. exists [].
-      eapply step_atomic with (t1:=[]). 1,2: reflexivity. cbn.
-      eapply ectx_language.Ectx_step with (K:=[SeqCtx]). 1,2: reflexivity.
-      constructor. eapply step_exec_instr; eauto. rewrite Hr //.
-    }
-    { simplify_eq. apply isCorrectPCb_nisCorrectPC in HPC.
-      eexists. eapply rtc_l. unfold erased_step. exists [].
-      eapply step_atomic with (t1:=[]). 1,2: reflexivity. cbn.
-      eapply ectx_language.Ectx_step with (K:=[SeqCtx]). 1,2: reflexivity. cbn.
-      constructor. eapply step_exec_corrfail; eauto.
-      eapply rtc_once. exists [].
-      eapply step_atomic with (t1:=[]). 1,2: reflexivity. cbn.
-      eapply ectx_language.Ectx_step with (K:=[]). 1,2: reflexivity. cbn.
-      constructor. }
-    { eexists. eapply rtc_once. exists [].
-      eapply step_atomic with (t1:=[]). 1,2: reflexivity. cbn.
-      eapply ectx_language.Ectx_step with (K:=[]). 1,2: reflexivity. cbn.
-      econstructor. }
-    { eexists. eapply rtc_once. exists [].
-      eapply step_atomic with (t1:=[]). 1,2: reflexivity. cbn.
-      eapply ectx_language.Ectx_step with (K:=[]). 1,2: reflexivity. cbn.
-      econstructor. }
-    { apply IHfuel in Hc as [φ' Hc]. eexists.
-      eapply rtc_l. exists [].
-      eapply step_atomic with (t1:=[]). 1,2: reflexivity. cbn.
-      eapply ectx_language.Ectx_step with (K:=[]). 1,2: reflexivity. cbn.
-      econstructor. cbn. apply Hc. } }
-Qed.
+      destruct (isCorrectPCb wpc) eqn:HPC.
+      { apply isCorrectPCb_isCorrectPC in HPC.
+        destruct wpc eqn:Hr; [by inversion HPC|].
+        destruct (m !! a) as [wa | ] eqn:HeMem.
+        2: {
+          eexists. eapply rtc_l. unfold erased_step. exists [].
+          eapply step_atomic with (t1:=[]). 1,2: reflexivity. cbn.
+          eapply ectx_language.Ectx_step with (K:=[SeqCtx]). 1,2: reflexivity. cbn.
+          constructor. eapply step_exec_memfail; eauto.
+          eapply rtc_once. exists []. simplify_eq.
+          eapply step_atomic with (t1:=[]). 1,2: reflexivity. cbn.
+          eapply ectx_language.Ectx_step with (K:=[]). 1,2: reflexivity. cbn.
+          constructor. }
+        eapply IHfuel in Hc as [φ' Hc]. eexists.
+        eapply rtc_l. unfold erased_step. exists [].
+        eapply step_atomic with (t1:=[]). 1,2: reflexivity. cbn.
+        eapply ectx_language.Ectx_step with (K:=[SeqCtx]). 1,2: reflexivity.
+        constructor. eapply step_exec_instr; eauto. rewrite Hr //.
+      }
+      { simplify_eq. apply isCorrectPCb_nisCorrectPC in HPC.
+        eexists. eapply rtc_l. unfold erased_step. exists [].
+        eapply step_atomic with (t1:=[]). 1,2: reflexivity. cbn.
+        eapply ectx_language.Ectx_step with (K:=[SeqCtx]). 1,2: reflexivity. cbn.
+        constructor. eapply step_exec_corrfail; eauto.
+        eapply rtc_once. exists [].
+        eapply step_atomic with (t1:=[]). 1,2: reflexivity. cbn.
+        eapply ectx_language.Ectx_step with (K:=[]). 1,2: reflexivity. cbn.
+        constructor. }
+      { eexists. eapply rtc_once. exists [].
+        eapply step_atomic with (t1:=[]). 1,2: reflexivity. cbn.
+        eapply ectx_language.Ectx_step with (K:=[]). 1,2: reflexivity. cbn.
+        econstructor. }
+      { eexists. eapply rtc_once. exists [].
+        eapply step_atomic with (t1:=[]). 1,2: reflexivity. cbn.
+        eapply ectx_language.Ectx_step with (K:=[]). 1,2: reflexivity. cbn.
+        econstructor. }
+      { apply IHfuel in Hc as [φ' Hc]. eexists.
+        eapply rtc_l. exists [].
+        eapply step_atomic with (t1:=[]). 1,2: reflexivity. cbn.
+        eapply ectx_language.Ectx_step with (K:=[]). 1,2: reflexivity. cbn.
+        econstructor. cbn. apply Hc. } }
+  Qed.
 
-Lemma machine_run_ends_in_halted_or_error `{MachineParameters}:
-  ∀ n init c, machine_run n init = Some c ->
-  c = Halted \/ c = Failed.
-Proof.
-  intros n.
-  induction n; intros init c mr.
-  - discriminate mr.
-  - simpl in mr.
-    destruct init as [[ | | | ] [r m]].
-    destruct (r !! PC).
-    destruct (isCorrectPCb w).
-    destruct (m !! match w with
-    | WInt _ => finz.largest 0%a
-    | WCap _ _ _ a => a
-    end). apply IHn in mr. apply mr.
-    1,2,3,5: right; symmetry; apply Some_inj in mr; apply mr.
-    left; symmetry. apply Some_inj in mr; apply mr.
-    apply IHn in mr. apply mr.
-Qed.
+  Lemma machine_run_ends_in_halted_or_error:
+    ∀ {n init c},
+      machine_run n init = Some c ->
+      c = Halted \/ c = Failed.
+  Proof.
+    intros n.
+    induction n; intros init c mr.
+    - discriminate mr.
+    - simpl in mr.
+      destruct init as [[ | | | ] [r m]].
+      destruct (r !! PC).
+      destruct (isCorrectPCb w).
+      destruct (m !! match w with
+      | WInt _ => finz.largest 0%a
+      | WCap _ _ _ a => a
+      end). apply IHn in mr. apply mr.
+      1,2,3,5: right; symmetry; apply Some_inj in mr; apply mr.
+      left; symmetry. apply Some_inj in mr; apply mr.
+      apply IHn in mr. apply mr.
+  Qed.
 
-Lemma machine_run_ends_incr `{MachineParameters}:
-  ∀ n' n init c,
-    n <= n' ->
-    machine_run n init = Some c ->
-    machine_run n' init = Some c.
-Proof.
-  induction n'.
-  - intros n init c n_inf_0. apply le_n_0_eq in n_inf_0.
-    rewrite n_inf_0. auto.
-  - intros n [ conf [r m] ] c n_inf_n'.
-    apply PeanoNat.Nat.le_succ_r in n_inf_n'.
-    destruct n_inf_n' as [n_inf_n' | n_eq_n'].
-    2: { rewrite n_eq_n'. auto. }
-    destruct n as [ | n ]. intros mr_n. discriminate mr_n.
-    simpl.
-    destruct conf.
-    destruct (r !! PC).
-    destruct (isCorrectPCb w).
-    destruct (m !! match w with
-    | WInt _ => finz.largest 0%a
-    | WCap _ _ _ a => a
-    end).
-    all: try auto.
-    all: apply IHn'; lia.
-Qed.
+  Lemma machine_run_ends_incr:
+    ∀ {n n' init c},
+      n <= n' ->
+      machine_run n init = Some c ->
+      machine_run n' init = Some c.
+  Proof.
+    intros n n'. generalize n. clear n.
+    induction n'.
+    - intros n init c n_inf_0. apply le_n_0_eq in n_inf_0.
+      rewrite n_inf_0. auto.
+    - intros n [ conf [r m] ] c n_inf_n'.
+      apply PeanoNat.Nat.le_succ_r in n_inf_n'.
+      destruct n_inf_n' as [n_inf_n' | n_eq_n'].
+      2: { rewrite n_eq_n'. auto. }
+      destruct n as [ | n ]. intros mr_n. discriminate mr_n.
+      simpl.
+      destruct conf.
+      destruct (r !! PC).
+      destruct (isCorrectPCb w).
+      destruct (m !! match w with
+      | WInt _ => finz.largest 0%a
+      | WCap _ _ _ a => a
+      end).
+      all: try auto.
+      all: apply IHn'; lia.
+  Qed.
+
+  Lemma machine_run_unique_result:
+    ∀ {n n' c c' init},
+      machine_run n init = Some c ->
+      machine_run n' init = Some c' ->
+      c = c'.
+  Proof.
+    intros n n' c c' init mr mr'.
+    destruct (le_lt_dec n n') as [nn' | nn'].
+    2: apply Nat.lt_le_incl in nn'.
+    rewrite (machine_run_ends_incr nn' mr) in mr'.
+    2: rewrite (machine_run_ends_incr nn' mr') in mr.
+    apply Some_inj in mr'. apply mr'.
+    apply Some_inj in mr. symmetry. apply mr.
+  Qed.
+
+End machine_run.
